\begin{equation*}
    \begin{split}
        \sum_{t=0}^{1} (-1)^t \binom{1}{t} n^{1-t} \sum_{k=1}^{n} k^{t+1} =& 1/6 (-n + n^3) \\
        \sum_{t=0}^{2} (-1)^t \binom{2}{t} n^{2-t} \sum_{k=1}^{n} k^{t+2} =& 1/30 (-n + n^5) \\
        \sum_{t=0}^{3} (-1)^t \binom{3}{t} n^{3-t} \sum_{k=1}^{n} k^{t+3} =& 1/420 (-10 n + 7 n^3 + 3 n^7) \\
        \sum_{t=0}^{4} (-1)^t \binom{4}{t} n^{4-t} \sum_{k=1}^{n} k^{t+4} =& 1/630 (-21 n + 20 n^3 + n^9) \\
        \sum_{t=0}^{5} (-1)^t \binom{5}{t} n^{5-t} \sum_{k=1}^{n} k^{t+5} =& 1/2772 (-210 n + 231 n^3 - 22 n^5 + n^{11}) \\
    \end{split}
\end{equation*}