Let be an example for $m=2$ of
\begin{equation*}
    \sum_{r=0}^{m} \coeffA{m}{r} \left[ \frac{1}{(2r+1) \binom{2r}r} n^{2r+1} \right]
    + 2 \sum_{r=0}^{m} \coeffA{m}{r} \left[ \sum_{d=0}^{(r-1)/2} \frac{(-1)^r}{2r-2d} \binom{r}{2d+1} \bernoulli{2r-2d} n^{2d+1} \right]
    - n^{2m+1} = 0
\end{equation*}
So that
\begin{equation*}
    \sum_{r=0}^{2} \coeffA{2}{r} \left[ \frac{1}{(2r+1) \binom{2r}r} n^{2r+1} \right]
    + 2 \sum_{r=0}^{2} \coeffA{2}{r} \left[ \sum_{d=0}^{(r-1)/2} \frac{(-1)^r}{2r-2d} \binom{r}{2d+1} \bernoulli{2r-2d} n^{2d+1} \right]
    - n^{5} = 0
\end{equation*}
The sum $\sum_{r=0}^{2} \coeffA{2}{r} \left[ \frac{1}{(2r+1) \binom{2r}r} n^{2r+1} \right]$ in explicit form is
\begin{equation*}
    \sum_{r=0}^{2} \coeffA{2}{r} \left[ \frac{1}{(2r+1) \binom{2r}r} n^{2r+1} \right] =
    \coeffA{2}{0} n
    + \coeffA{2}{1} \left[ \frac{1}{3 \binom{2}{1}} n^{3} \right]
    + \coeffA{2}{2} \left[ \frac{1}{5 \binom{4}{2}} n^{5} \right]
\end{equation*}
Also the sum
$\sum_{r=0}^{2} \coeffA{2}{r} \left[ \sum_{d=0}^{(r-1)/2} \frac{(-1)^r}{2r-2d} \binom{r}{2d+1} \bernoulli{2r-2d} n^{2d+1} \right]$
is
\begin{equation*}
    \begin{split}
        &\sum_{r=0}^{2} \coeffA{2}{r} \left[ \sum_{d=0}^{(r-1)/2} \frac{(-1)^r}{2r-2d} \binom{r}{2d+1} \bernoulli{2r-2d} n^{2d+1} \right] = \\
        & + \coeffA{2}{0} \left[ \sum_{d=0}^{-1} \frac{1}{-2d} \binom{0}{2d+1} \bernoulli{-2d} n^{2d+1} \right] \\
        & - \coeffA{2}{1} \left[ \sum_{d=0}^{0} \frac{1}{2-2d} \binom{1}{2d+1} \bernoulli{2-2d} n^{2d+1} \right] \\
        & + \coeffA{2}{2} \left[ \sum_{d=0}^{0} \frac{1}{4-2d} \binom{2}{2d+1} \bernoulli{4-2d} n^{2d+1} \right] \\
        & = \coeffA{2}{0} \cdot 0
        - \coeffA{2}{1} \left[ \frac{1}{2} \binom{1}{1} \bernoulli{2} n^{1} \right]
        + \coeffA{2}{2} \left[ \frac{1}{4} \binom{2}{1} \bernoulli{4} n^{1} \right] \\
        & = \coeffA{2}{0} \cdot 0
        - \coeffA{2}{1} \left[ \frac{1}{12} n \right]
        - \coeffA{2}{2} \left[ \frac{1}{60} n \right] \\
        & = - \coeffA{2}{1} \frac{1}{12} n
        - \coeffA{2}{2}  \frac{1}{60} n
    \end{split}
\end{equation*}
