For $m=2$ we have an identity

\begin{equation*}
    \coeffA{m}{0} n
    + \coeffA{m}{1} \left[ \frac{1}{6} (-n + n^3) \right]
    + \coeffA{m}{2} \left[ \frac{1}{30} (-n + n^5) \right] - n^5 = 0
\end{equation*}
Multiplying by 30 both parts we get
\begin{equation*}
    30 \coeffA{m}{0} n
    + 5 \coeffA{m}{1}  (-n + n^3)
    + \coeffA{m}{2} (-n + n^5) - 30 n^5 = 0
\end{equation*}

Opening brackets gives
\begin{equation*}
    30 \coeffA{m}{0} n -5 \coeffA{m}{1} n + 5 \coeffA{m}{1} n^3 -\coeffA{m}{2} n + n^5 \coeffA{m}{2} n^5 - 30 n^5 = 0
\end{equation*}

Arranging terms we get

\begin{equation*}
    n (30 \coeffA{m}{0} n - 5 \coeffA{m}{1} -\coeffA{m}{2}) + 5 \coeffA{m}{1} n^3 + n^5 (\coeffA{m}{2} n^5 - 30) = 0, \quad n \geq 1
\end{equation*}

Hence

\begin{equation*}
    \begin{cases}
        \coeffA{m}{1} = 0 \\
        \coeffA{m}{2} n^5 - 30 = 0 \\
        30 \coeffA{m}{0} n - 5 \coeffA{m}{1} -\coeffA{m}{2} = 0
    \end{cases}
\end{equation*}

So that $\coeffA{m}{1}=6 \quad \coeffA{m}{1} = 1$