\begin{equation*}
    \begin{split}
        \sum_{k=1}^{n} k^{1} &= 1/2 (-n + n^2) \\
        \sum_{k=1}^{n} k^{2} &= 1/6 (n - 3 n^2 + 2 n^3) \\
        \sum_{k=1}^{n} k^{3} &= 1/4 (n^2 - 2 n^3 + n^4) \\
        \sum_{k=1}^{n} k^{4} &= 1/30 (-n + 10 n^3 - 15 n^4 + 6 n^5) \\
        \sum_{k=1}^{n} k^{5} &= 1/12 (-n^2 + 5 n^4 - 6 n^5 + 2 n^6) \\
        \sum_{k=1}^{n} k^{6} &= 1/42 (n - 7 n^3 + 21 n^5 - 21 n^6 + 6 n^7) \\
        \sum_{k=1}^{n} k^{7} &= 1/24 (2 n^2 - 7 n^4 + 14 n^6 - 12 n^7 + 3 n^8) \\
        \sum_{k=1}^{n} k^{8} &= 1/90 (-3 n + 20 n^3 - 42 n^5 + 60 n^7 - 45 n^8 + 10 n^9) \\
    \end{split}
\end{equation*}