\begin{examp}
    Let be fixed $m=2$ so that we have the following relation defined by (eqref)
    \begin{equation*}
        \coeffA{m}{0} n
        + \coeffA{m}{1} \left[ \frac{1}{6} (-n + n^3) \right]
        + \coeffA{m}{2} \left[ \frac{1}{30} (-n + n^5) \right] - n^5 = 0
    \end{equation*}
\end{examp}
Multiplying by $30$ both, right hand side and left hand side, we get
\begin{equation*}
    30 \coeffA{2}{0} n + 5 \coeffA{2}{1} (-n + n^3) + \coeffA{2}{2} (-n + n^5) - 30n^5 = 0
\end{equation*}
Opening brackets and rearranging the terms gives
\begin{equation*}
    30 \coeffA{2}{0} - 5 \coeffA{2}{1} n + 5 \coeffA{2}{1} n^3 - \coeffA{2}{2} n + \coeffA{2}{2} n^5 - 30n^5 = 0
\end{equation*}
Combining the terms yields
\begin{equation*}
    n (30 \coeffA{2}{0} - 5 \coeffA{2}{1} - \coeffA{2}{2}) + 5 \coeffA{2}{1} n^3 + n^5 (\coeffA{2}{2} - 30) = 0
\end{equation*}
Therefore, the system of linear equations follows
\begin{equation*}
    \begin{cases}
        30 \coeffA{2}{0} - 5 \coeffA{2}{1} - \coeffA{2}{2} = 0 \\
        \coeffA{2}{1} = 0 \\
        \coeffA{2}{2} - 30 = 0
    \end{cases}
\end{equation*}
Solving it we get
\begin{equation*}
    \begin{cases}
        \coeffA{2}{2} = 30 \\
        \coeffA{2}{1} = 0 \\
        \coeffA{2}{0} = 1
    \end{cases}
\end{equation*}