For $m=1$ we have an identity

\begin{equation*}
    \coeffA{m}{0} n + \coeffA{m}{1} \left[ \frac{1}{6} (-n + n^3) \right] - n^3 = 0
\end{equation*}
Multiplying by 6 both parts we get
\begin{equation*}
    6 \coeffA{m}{0} n + \coeffA{m}{1} (-n + n^3)  - 6 n^3 = 0
\end{equation*}

Opening brackets gives
\begin{equation*}
    6 \coeffA{m}{0} n - \coeffA{m}{1} n + \coeffA{m}{1} n^3  - 6 n^3 = 0
\end{equation*}

Arranging terms we get

\begin{equation*}
    n (6\coeffA{m}{0} - \coeffA{m}{1})+ n^3 (\coeffA{m}{1} - 6)  = 0, \quad n \geq 1
\end{equation*}

Hence

\begin{equation*}
    \begin{cases}
        6\coeffA{m}{0} - \coeffA{m}{1} = 0 \\
        \coeffA{m}{1} - 6 = 0
    \end{cases}
\end{equation*}

So that $\coeffA{m}{1}=6 \quad \coeffA{m}{1} = 1$